src/lowparse/LowParse.Low.VLData.Aux.fst
@@ -1,0 +1,46 @@
+module LowParse.Low.VLData.Aux
+open LowParse.Low.Combinators
+
+module B = LowStar.Buffer
+module E = LowParse.BigEndianImpl.Low
+module HST = FStar.HyperStack.ST
+
+inline_for_extraction
+let parse32_bounded_integer_1 _ : (parser32 (parse_bounded_integer 1)) =
+  decode_bounded_integer_injective 1;
+  make_total_constant_size_parser32 1 1ul #(bounded_integer 1) (decode_bounded_integer 1) () (fun input ->
+    let h = HST.get () in
+    let r = E.be_to_n_1 _ _ (E.u32 ()) input in
+    E.lemma_be_to_n_is_bounded (B.as_seq h input);
+    r
+  )
+
+inline_for_extraction
+let parse32_bounded_integer_2 _ : (parser32 (parse_bounded_integer 2)) =
+  decode_bounded_integer_injective 2;
+  make_total_constant_size_parser32 2 2ul #(bounded_integer 2) (decode_bounded_integer 2) () (fun input ->
+    let h = HST.get () in
+    let r = E.be_to_n_2 _ _ (E.u32 ()) input in
+    E.lemma_be_to_n_is_bounded (B.as_seq h input);
+    r
+  )
+
+inline_for_extraction
+let parse32_bounded_integer_3 _ : (parser32 (parse_bounded_integer 3)) =
+  decode_bounded_integer_injective 3;
+  make_total_constant_size_parser32 3 3ul #(bounded_integer 3) (decode_bounded_integer 3) () (fun input ->
+    let h = HST.get () in
+    let r = E.be_to_n_3 _ _ (E.u32 ()) input in
+    E.lemma_be_to_n_is_bounded (B.as_seq h input);
+    r
+  )
+
+inline_for_extraction
+let parse32_bounded_integer_4 _ : (parser32 (parse_bounded_integer 4)) =
+  decode_bounded_integer_injective 4;
+  make_total_constant_size_parser32 4 4ul #(bounded_integer 4) (decode_bounded_integer 4) () (fun input ->
+    let h = HST.get () in
+    let r = E.be_to_n_4 _ _ (E.u32 ()) input in
+    E.lemma_be_to_n_is_bounded (B.as_seq h input);
+    r
+  )
