src/lowparse/LowParse.Low.VLData.Aux.fsti
@@ -1,0 +1,15 @@
+module LowParse.Low.VLData.Aux
+include LowParse.Spec.VLData
+include LowParse.Low.Base
+
+inline_for_extraction
+val parse32_bounded_integer_1 : unit -> Tot (parser32 (parse_bounded_integer 1))
+
+inline_for_extraction
+val parse32_bounded_integer_2 : unit -> Tot (parser32 (parse_bounded_integer 2))
+
+inline_for_extraction
+val parse32_bounded_integer_3 : unit -> Tot (parser32 (parse_bounded_integer 3))
+
+inline_for_extraction
+val parse32_bounded_integer_4 : unit -> Tot (parser32 (parse_bounded_integer 4))
